\documentclass{article}

\usepackage{physics,amsmath,geometry,amsfonts,wrapfig,graphicx,array,makecell,float,enumitem,bm}

\title{Question 1}
\author{Yue Wu}

\geometry{a4paper,hmargin=1.1in,vmargin=1.2in}

\setlength{\parindent}{0pt}
\setlength{\parskip}{1em}

\begin{document}
    \begin{center}
        \LARGE\textbf{Post-Lecture Question 1}
    \end{center}

    \begin{enumerate}
        \item[(a)]
        $$\dd{E}=T\dd{S}-p\dd{V}+\mu\dd{N}$$
        \begin{align*}
            \qty(\pdv{E}{S})_{V,N}=T\quad&\Rightarrow\quad\qty(\pdv{S}{E})_{V,N}=\frac{1}{T}\\
            T\qty(\pdv{S}{N})_{E,V}+\mu=0\quad&\Rightarrow\quad\qty(\pdv{S}{N})_{E,V}=-\frac{\mu}{T}
        \end{align*}
        \item[(b)]
        \begin{align*}
            &\ln\Omega_{\text{bath}}(N-N_S,E-E_S)\\
            =&\ln\Omega_{\text{bath}}(N,E)-N_S\qty(\pdv{\ln\Omega_{\text{bath}}}{N})_E (N,E)-E_S\qty(\pdv{\ln\Omega_{\text{bath}}}{E})_N (N,E)+\mathcal{O}(N_S^{n}E_S^{2-n})\\
            =&\ln\Omega_{\text{bath}}(N,E)-\frac{N_S}{k_B}\qty(\pdv{S}{N})_E-\frac{E_S}{k_B}\qty(\pdv{S}{E})_N\\
            =&\ln\Omega_{\text{bath}}(N,E)-\beta E_S+\beta N_S\mu
        \end{align*}
        \item[(c)]
        $$\exp(\ln\Omega_{\text{bath}}(N-N_S,E-E_S))=\Omega_{\text{bath}}(N,E)e^{-\beta E_S}e^{\beta N_S\mu}$$
        \begin{align*}
            \Rightarrow\quad P(N_S,E_S)&=\frac{\Omega_{\text{bath}}(N,E)e^{-\beta E_S}e^{\beta N_S\mu}}{\sum_i\sum_j\Omega_{\text{bath}}(N,E)e^{-\beta E_j}e^{\beta N_i\mu}}\\
            &=\frac{e^{-\beta E_S}e^{\beta N_S\mu}}{\sum_i\sum_j e^{-\beta E_j}e^{\beta N_i\mu}}
        \end{align*}
        \begin{align*}
            P(N_S)&=\frac{\sum_j e^{-\beta E_j}e^{\beta N_S\mu}}{\sum_i\sum_j e^{-\beta E_j}e^{\beta N_i\mu}}\\
            &=\frac{Q(N_S,V,T)e^{\beta N_S\mu}}{\sum_{N=0}^{\infty}Q(N,V,T)e^{\beta N\mu}}
        \end{align*}
    \end{enumerate}

\end{document}