\documentclass{article}

\usepackage{physics,amsmath,geometry,amsfonts,wrapfig,graphicx,array,makecell,float,enumitem,bm}

\title{Question 3}
\author{Yue Wu}

\geometry{a4paper,hmargin=1.1in,vmargin=1.2in}

\setlength{\parindent}{0pt}
\setlength{\parskip}{1em}

\begin{document}
    \begin{center}
        \LARGE\textbf{Post-Lecture Question 3}
    \end{center}

    \begin{enumerate}
        \item[(a)]
        \begin{enumerate}
            \item[(i)] $U(\{\vb{r}_i\})=0$
            $$Q=\frac{1}{\Lambda^{3N}N!}\int\prod_{i=1}^{N}\dd{\vb{r}_i}=\frac{V^N}{\Lambda^{3N}N!}$$
            
            \item[(ii)]
            \begin{enumerate}
                \item[($\alpha$)]
                \begin{align*}
                    A&=-k_BT\ln Q\\
                    &=-Nk_BT\ln V+3Nk_B T\ln\Lambda+k_B T\ln N!\\
                    &\approx -Nk_BT\ln V+3Nk_BT\ln\Lambda+Nk_BT\ln N-Nk_BT\\
                    &=Nk_BT\qty[\ln\frac{N\Lambda^3}{V}-1]
                \end{align*}
                \item[($\beta$)]
                $$\ln Q=N\ln V-3N\ln\Lambda-\ln N!$$
                $$E=-\qty(\pdv{\ln Q}{\beta})_{N,V}=3N\qty(\pdv{\ln\Lambda}{\beta})_{N,V}$$
                $$\Lambda=\frac{h}{\sqrt{2\pi mk_B T}}=\frac{h}{\sqrt{2\pi m}}\beta^{\frac{1}{2}}\quad\Rightarrow\quad\qty(\pdv{\ln\Lambda}{\beta})_{N,V}=\frac{1}{2\beta}$$
                $$E=\frac{3}{2}Nk_B T$$
                \item[($\gamma$)]
                $$S=\frac{E-A}{T}=Nk_B\qty[\frac{5}{2}+\ln\frac{V}{N\Lambda^3}]$$
                \item[($\delta$)] 
                \begin{align*}
                    P&=-\qty(\pdv{A}{V})_{T,\mu}\\
                    &=Nk_BT\pdv{V}\ln V=\frac{Nk_BT}{V}
                \end{align*}
            \end{enumerate}
            \item[(iii)]
            $$S=Nk_B\qty(\frac{5}{2}+\ln\frac{V}{N}-3\ln\Lambda)$$
            $$\lim_{T\to 0}\Lambda=\frac{h}{\sqrt{2\pi mk_BT}}=\infty$$
            $$\Rightarrow\quad\lim_{T\to 0^+}S=-\infty$$
            \item[(iv)]
            \begin{align*}
                \mu&=\qty(\pdv{A}{N})_{V,T}=k_BT\qty[\ln\frac{N\Lambda^3}{V}-1]+Nk_BT\frac{V}{N\Lambda^3}\frac{\Lambda^3}{V}\\
                &=k_BT\ln\frac{N\Lambda^3}{V}-k_BT+k_BT\\
                &=k_BT\ln\rho\Lambda^3
            \end{align*}
        \end{enumerate}
        \item[(b)]
        \begin{align*}
            PV&=k_BT\ln\Xi\\
            &=k_BT\ln\sum_{N=0}^{\infty}\frac{z^NV^N}{\Lambda^{3N}N!}\\
            &=k_BT\ln\sum_{N=0}^{\infty}\frac{1}{N!}(\frac{zV}{\Lambda^3})^N\\
            &=k_BT\frac{zV}{\Lambda^3}
        \end{align*}
        Have
        $$\expval{N}=\qty(\pdv{\ln\Xi}{\beta\mu})_{V,T}=\pdv{\beta\mu}\frac{zV}{\Lambda^3}=\frac{zV}{\Lambda^3}\,.$$
        Therefore,
        $$PV=\expval{N}k_BT\,,$$
        consistent with (a)(ii)($\delta$).
        \item[(c)]
        \begin{enumerate}
            \item[(i)]
            \begin{align*}
                \Delta&=\beta P\int_{0}^{\infty}\frac{1}{\Lambda^{3N}N!}V^N e^{-\beta PV}\dd{V}\\
                &=\frac{1}{\Lambda^{3N}N!(\beta P)^N}\int_{0}^{\infty}(\beta PV)^N e^{-\beta PV}\dd{(\beta PV)}\\
                &=\frac{1}{\Lambda^{3N}N!(\beta P)^N}\Gamma(N+1)\\
                &=\frac{1}{\Lambda^{3N}(\beta P)^N}
            \end{align*}
            \item[(ii)]
            \begin{align*}
                G&=-k_BT\ln\Delta\\
                &=k_BT\ln\Lambda^{3N}(\beta P)^N\\
                &=Nk_BT\ln\beta P\Lambda^3
            \end{align*}
            \begin{align*}
                \mu&=\qty(\pdv{G}{N})_{P,T}\\
                &=k_BT\ln\beta P\Lambda^3
            \end{align*}
            Result from (a) and (b):
            \begin{align*}
                \mu&=k_BT\ln\frac{N}{V}\Lambda^3\\
                &=k_BT\ln\frac{P}{k_BT}\Lambda^3\\
                &=k_BT\ln\beta P\Lambda^3\,,
            \end{align*}
            which is consistent.
        \end{enumerate}
    \end{enumerate}

\end{document}