\documentclass{article}

\usepackage{physics,amsmath,geometry,amsfonts,wrapfig,graphicx,array,makecell,float,enumitem,bm}

\title{Question 2}
\author{Yue Wu}

\geometry{a4paper,hmargin=1.1in,vmargin=1.2in}

\setlength{\parindent}{0pt}
\setlength{\parskip}{1em}


\begin{document}
    \begin{center}
        \LARGE\textbf{Post-Lecture Question 2}
    \end{center}

    \begin{enumerate}
        \item[(a)]
        \begin{enumerate}
            \item[(i)]
            $$\dd{E}=T\dd{S}-p\dd{V}+\mu\dd{N}\quad\Rightarrow\quad\qty(\pdv{S}{N})_{E,V}=-\frac{\mu}{T}\,,\;\qty(\pdv{S}{E})_{N,V}=\frac{1}{T}\,.$$
            \begin{align*}
                S_{\text{bath}}&=k_B\ln\Omega_{\text{bath}}(N-N_S,E-E_S)\\
                &=k_B\qty[\ln\Omega_{\text{bath}}(N,E)-N_S\qty(\pdv{\ln\Omega_{\text{bath}}}{N})_{E,V}(N,E)-E_S\qty(\pdv{\ln\Omega_{\text{bath}}}{E})_{N,V}(N,E)]\\
                &=k_B\qty[\ln\Omega_{\text{bath}}(N,E)-\frac{N_S}{k_B}\qty(\pdv{S_{\text{bath}}}{N})_{E,V}(N,E)-\frac{E_S}{k_B}\qty(\pdv{S_{\text{bath}}}{E})_{N,V}(N,E)]\\
                &=S_{\text{bath}}(N,E)-\frac{\mu_{\text{bath}N_S}}{T_{\text{bath}}}-\frac{E_S}{T_{\text{bath}}}
            \end{align*}
            $$\Rightarrow\quad S_{\text{total}}=S_{\text{bath}}(N,E)+S_{\text{sys}}(N_S,E_S)+\frac{1}{T_{\text{bath}}}(\mu_{\text{bath}}N_S-E_S)$$
            When $S_{\text{total}}$ is maximised,
            \begin{align*}
                \pdv{S_{\text{total}}}{N_S}&=\pdv{S_{\text{sys}}}{N_S}(N_S,E_S)+\frac{\mu_{\text{bath}}}{T_{\text{bath}}}\\
                &=-\frac{\mu_{\text{sys}}}{T_{\text{sys}}}+\frac{\mu_{\text{bath}}}{T_{\text{bath}}}=0\\
                \pdv{S_{\text{total}}}{E_S}&=\pdv{S_{\text{sys}}}{E_S}(N_S,E_S)-\frac{1}{T_{\text{bath}}}\\
                &=\frac{1}{T_{\text{sys}}}-\frac{1}{T_{\text{bath}}}=0\\
            \end{align*}
            $$\Rightarrow\quad\left\{\begin{aligned}
                T_\text{sys}=T_\text{bath}=T\\
                \mu_\text{sys}=\mu_\text{bath}=\mu
            \end{aligned}\right.$$
            \begin{align*}
                \Phi_{\text{sys}}(N_S,E_S)&=E_S-TS_{\text{sys}}(N_S,E_S)-N_S\mu\\
                &=-T\qty[S_{\text{sys}}(N_S,E_S)+\frac{1}{T}(N_S\mu-E_S)]\\
                &=-TS_{\text{total}}+TS_{\text{bath}}(N,E)\,,
            \end{align*}
            where $TS_{\text{bath}}(N,E)$ is a constant. As $T>0$, maximum $S_{\text{total}}\Rightarrow$ minimum $\Phi_{\text{sys}}$.
            \item[(ii)] At fixed $T,\mu$, $\dd{\Phi}=-P\dd{V}\Rightarrow\Phi=-PV$. As $V_{\text{sys}}$ fixed and $V,P>0$, $\Phi_{\text{sys}}$ is minimised by maximum $P_{\text{sys}}$.
            
        \end{enumerate}
        \item[(b)]
        \begin{enumerate}
            \item[(i)]
            \begin{align*}
                \qty(\pdv{Q}{\beta})_{N,V}&=\pdv{\beta}\sum_i e^{-\beta E_i}=-\sum_iE_ie^{-\beta E_i}\\
                &=-\sum_i e^{-\beta E_i}\frac{\sum_j E_j e^{-\beta E_j}}{\sum_k e^{-\beta E_k}}\\
                &=-Q\expval{E}_N
            \end{align*}
            \item[(ii)] Have
            $$\Xi=\sum_i\sum_j e^{-\beta E_i}z^{N_j}\,.$$
            \begin{align*}
                \qty(\pdv{\ln\Xi}{\beta})_{z,V}&=\frac{1}{\Xi}\qty(\pdv{\xi}{\beta})_{z,V}\\
                &=\frac{1}{\Xi}\sum_i\sum_j\pdv{\beta}e^{-\beta E_i}z^{N_j}\\
                &=-\frac{1}{\Xi}\sum_i\sum_j E_i e^{-\beta E_i}z^{N_j}
            \end{align*}
            \begin{align*}
                \expval{E}&=\sum_i\sum_jE_i P(E_i,N_j)\\
                &=\sum_i\sum_jE_i\frac{e^{-\beta E_i}z^{N_j}}{\sum_p\sum_q e^{-\beta E_p}z^{N_q}}\\
                &=\frac{1}{\Xi}\sum_i\sum_jE_i e^{-\beta E_i}z^{N_j}\\
                &=-\qty(\pdv{\ln\Xi}{\beta})_{z,V}
            \end{align*}
            \item[(iii)]
            $$\Xi=\sum_i\sum_j e^{-\beta E_i}e^{\beta\mu N_j}$$
            \begin{align*}
                \qty(\pdv{\ln\Xi}{\beta})_{\mu,V}&=\frac{1}{\Xi}\qty(\pdv{\xi}{\beta})_{\mu,V}\\
                &=\frac{1}{\Xi}\qty(\sum_i\sum_j-E_ie^{-\beta E_i}e^{\beta\mu N_j}+\sum_i\sum_j\mu N_j e^{-\beta E_i}e^{\beta\mu N_j})\\
                &=-\frac{1}{\Xi}\sum_i\sum_j E_ie^{-\beta E_i}e^{\beta\mu N_j}+\mu\frac{1}{\Xi}\sum_i\sum_j N_j e^{-\beta E_i}e^{\beta\mu N_j}\\
                &=-\expval{E}+\mu\expval{N}
            \end{align*}
            \item[(iv)]
            \begin{align*}
                \qty(\pdv{(\Phi/T)}{(1/T)})_{\mu,V}&=\frac{1}{T}\qty(\pdv{\Phi}{(1/T)})_{\mu,V}+\Phi\qty(\pdv{(1/T)}{(1/T)})_{\mu,V}\\
                &=\frac{1}{T}\qty(\pdv{\Phi}{T})_{\mu,V}\qty[\pdv{T}\frac{1}{T}]^{-1}+\Phi\\
                &=-TS+E-TS-\mu N\\
                &=E-\mu N
            \end{align*}
            \item[(v)] In the thermodynamic limit, $E=\expval{E}$ and $N=\expval{N}$, so
            $$\qty(\pdv{(\beta\Phi)}{\beta})_{\mu,V}=\qty(\pdv{(\Phi/T)}{(1/T)})_{\mu,V}=-\qty(\pdv{\ln\Xi}{\beta})_{\mu,V}$$
            $$\Rightarrow \beta\Phi=-\ln\Xi+c$$
            Set $c=0$, get $\Phi=-k_B T\ln\Xi$.
        \end{enumerate}
    \end{enumerate}

\end{document}