\documentclass{article}

\usepackage{physics,amsmath,geometry,amsfonts,wrapfig,graphicx,array,makecell,float,enumitem,bm,tikz}

\title{Question 5}
\author{Yue Wu}

\geometry{a4paper,hmargin=0.8in,vmargin=1in}

\setlength{\parindent}{0pt}
\setlength{\parskip}{1em}

\begin{document}
    \begin{center}
        \LARGE\textbf{Post-Lecture Question 5}
    \end{center}

    \begin{enumerate}
        \item[(a)]
        \begin{align*}
            \beta A(\lambda)&=-\ln Q(\lambda)\\
            &=\ln(\Lambda^{3N} N!)-\ln\int\prod_{i=1}^{N}\dd{\vb{r}_i}\exp(-\beta U(\{\vb{r}_i\};\lambda))
        \end{align*}
        \item[(b)]
        \begin{align*}
            \qty(\pdv{A}{\lambda})_{N,V,T}&=-\frac{1}{\beta}\pdv{\lambda}\ln\int\prod_{i=1}^{N}\dd{\vb{r}_i}\exp(-\beta U(\{\vb{r}_i\};\lambda))\\
            &=-\frac{\int\prod_{i=1}^{N}\dd{\vb{r}_i}\pdv{\lambda}\exp(-\beta U(\{\vb{r}_i\};\lambda))}{\beta\int\prod_{i=1}^{N}\dd{\vb{r}_i}\exp(-\beta U(\{\vb{r}_i\};\lambda))}\\
            &=\frac{\int\prod_{i=1}^{N}\dd{\vb{r}_i}\pdv{U(\{\vb{r}_i\};\lambda)}{\lambda}\exp(-\beta U(\{\vb{r}_i\};\lambda))}{\beta\int\prod_{i=1}^{N}\dd{\vb{r}_i}\exp(-\beta U(\{\vb{r}_i\};\lambda))}\\
            &=\expval{\qty(\pdv{U}{\lambda})_{N,V,T}}_\lambda
        \end{align*}
        \item[(c)]
        \begin{align*}
            A_1-A_0&=\int_{0}^{1}\dd{\lambda}\qty(\pdv{A}{\lambda})_{N,V,T}\\
            &=\int_{0}^{1}\dd{\lambda}\expval{\qty(\pdv{U}{\lambda})_{N,V,T}}_\lambda\\
            &=\int_{0}^{1}\dd{\lambda}\expval{-2(1-\lambda)U_0+2\lambda U_1}_\lambda
        \end{align*}
        \item[(d)]
        \begin{align*}
            \qty(\pdv[2]{A}{\lambda})_{N,V,T}&=\qty(\pdv{\lambda})_{N,V,T}\qty[\frac{\int\prod_{i=1}^{N}\dd{\vb{r}_i}\pdv{U}{\lambda}\exp(-\beta U(\{\vb{r}_i\};\lambda))}{\int\prod_{i=1}^{N}\dd{\vb{r}_i}\exp(-\beta U(\{\vb{r}_i\};\lambda))}]\\
            &=\frac{1}{\qty[\int\prod_{i=1}^{N}\dd{\vb{r}_i}\exp(-\beta U)]^2}\left[\qty(\int\prod_{i=1}^{N}\dd{\vb{r}_i}\pdv[2]{U}{\lambda}\exp(-\beta U)-\beta\int\prod_{i=1}^{N}\dd{\vb{r}_i}\qty(\pdv{U}{\lambda})^2\exp(-\beta U))\right.\\
            &\quad\left.\int\prod_{i=1}^{N}\dd{\vb{r}_i}\exp(-\beta U)+\beta\qty(\int\prod_{i=1}^{N}\dd{\vb{r}_i}\exp(-\beta U))^2\right]\\
            &=\frac{\int\prod_{i=1}^{N}\dd{\vb{r}_i}\pdv[2]{U}{\lambda}\exp(-\beta U)}{\int\prod_{i=1}^{N}\dd{\vb{r}_i}\exp(-\beta U)}-\beta\frac{\int\prod_{i=1}^{N}\dd{\vb{r}_i}\qty(\pdv{U}{\lambda})^2\exp(-\beta U)}{\int\prod_{i=1}^{N}\dd{\vb{r}_i}\exp(-\beta U)}+\beta\qty[\frac{\int\prod_{i=1}^{N}\dd{\vb{r}_i}\pdv{U}{\lambda}\exp(-\beta U)}{\int\prod_{i=1}^{N}\dd{\vb{r}_i}\exp(-\beta U)}]^2\\
            &=\expval{\pdv[2]{U}{\lambda}}_\lambda-\beta\expval{\qty[\qty(\pdv{U}{\lambda})_{N,V,T}]^2}_\lambda+\beta\expval{\qty(\pdv{U}{\lambda})_{N,V,T}}^2_\lambda
        \end{align*}
        $$\expval{\pdv[2]{U}{\lambda}}_\lambda=\expval{2U_0+2U_1}_\lambda$$
        $$\expval{\qty[\qty(\pdv{U}{\lambda})_{N,V,T}]^2}_\lambda=\expval{(-2(1-\lambda)U_0+2\lambda U_1)^2}_\lambda$$
        $$\expval{\qty(\pdv{U}{\lambda})_{N,V,T}}^2_\lambda=\expval{-2(1-\lambda)U_0+2\lambda U_1}^2_\lambda$$
        \item[(e)]
        \begin{align*}
            \pdv[2]{A}{\lambda}&=\expval{\pdv[2]{U}{\lambda}}_\lambda-\beta\qty[\expval{\qty[\qty(\pdv{U}{\lambda})_{N,V,T}]^2}_\lambda-\beta\expval{\qty(\pdv{U}{\lambda})_{N,V,T}}^2_\lambda]\\
            &=\expval{\pdv[2]{U}{\lambda}}_\lambda-\beta\sigma^2\qty(\qty(\pdv{U}{\lambda})_{N,V,T})\,,
        \end{align*}
        where the latter term is non-negative, while the former term has unknown sign. The Gibbs-Bogoliubov inequality does not hold.
    \end{enumerate}

\end{document}