\documentclass{article}

\usepackage{physics,amsmath,geometry,amsfonts,wrapfig,graphicx,array,makecell,float,enumitem,bm,tikz}

\title{Question 4}
\author{Yue Wu}

\geometry{a4paper,hmargin=1.1in,vmargin=1.2in}

\setlength{\parindent}{0pt}
\setlength{\parskip}{1em}

\begin{document}
    \begin{center}
        \LARGE\textbf{Post-Lecture Question 4}
    \end{center}

    \begin{enumerate}
        \item[(a)]
        $$\dd{E}=T\dd{S}-p\dd{V}+\mu\dd{N}$$
        $$\Rightarrow\quad\dd{S}=\frac{1}{T}\dd{E}+\frac{P}{T}\dd{V}-\frac{\mu}{T}\dd{N}$$
        \begin{align*}
            \dd{S}&=\dd{S}_\alpha+\dd{S}_\beta\\
            &=\frac{1}{T_\alpha}\dd{E}_\alpha+\frac{P_\alpha}{T_\alpha}\dd{V}_\alpha-\frac{\mu_{\alpha 1}}{T_{\alpha}}\dd{N}_{\alpha 1}-\frac{\mu_{\alpha 2}}{T_\alpha}\dd{N}_{\alpha 2}\\
            &\quad +\frac{1}{T_\beta}\dd{E}_\beta+\frac{P_\beta}{T_\beta}\dd{V}_\beta-\frac{\mu_{\beta 1}}{T_{\beta}}\dd{N}_{\beta 1}-\frac{\mu_{\beta 2}}{T_\beta}\dd{N}_{\beta 2}\\
            &=0
        \end{align*}
        Have
        \begin{align*}
            \dd{E}_\alpha=-\dd{E}_\beta\quad&\Rightarrow\quad\qty(\frac{1}{T_\alpha}-\frac{1}{T_\beta})\dd{E}_\alpha=0\\
            \dd{E}_\alpha=-\dd{E}_\beta\quad&\Rightarrow\quad\qty(\frac{1}{T_\alpha}-\frac{1}{T_\beta})\dd{E}_\alpha=0\\
            \dd{N}_{\alpha 1}=-\dd{N}_{\beta 1}\quad&\Rightarrow\quad\frac{1}{T}\qty(\mu_{\beta 1}-\mu_{\alpha 1})\dd{N}_{\beta 1}=0\\
            \dd{N}_{\alpha 2}=-\dd{N}_{\beta 2}\quad&\Rightarrow\quad\frac{1}{T}\qty(\mu_{\beta 2}-\mu_{\alpha 2})\dd{N}_{\beta 2}=0\\
        \end{align*}
        $$\Rightarrow\left\{\begin{aligned}
            &T_\alpha=T_\beta=T\\
            &P_\alpha=P_\beta=P\\
            &\mu_{\beta 1}=\mu_{\alpha 1}=\mu_1\\
            &\mu_{\beta 2}=\mu_{\alpha 2}=\mu_2\\
        \end{aligned}\right.$$

        It is unnecessary that $\mu_1=\mu_2$.
        \item[(b)]
        $$\left\{\begin{aligned}
            &T_\alpha=T_\beta=T_{\text{bath}}\\
            &P_\alpha=P_\beta=P_{\text{bath}}\\
            &\mu_{\beta 1}=\mu_{\alpha 1}\\
            &\mu_{\beta 2}=\mu_{\alpha 2}\\
        \end{aligned}\right.$$
        \item[(c)]
        $$\dd{G}=-S\dd{T}-V\dd{P}+\mu\dd{N}$$
        \begin{align*}
            \Delta G_1&=\frac{1}{2}\qty(\pdv[2]{G_1}{N_{\alpha 1}})_{N_2,T,P}(\Delta N_{\alpha 1})^2+\frac{1}{2}\qty(\pdv[2]{G_1}{N_{\beta 1}})_{N_2,T,P}(\Delta N_{\beta 1})^2\\
            &=\qty(\pdv[2]{G_1}{N_1})_{N_2,T,P}(\Delta N_1)^2\\
            &=\qty(\pdv{\mu_1}{N_1})_{N_2,T,P}(\Delta N_1)^2\ge 0
        \end{align*}
        $$\Rightarrow\quad\qty(\pdv{\mu_1}{N_1})_{N_2,T,P}\ge 0$$
    \end{enumerate}

\end{document}